\documentclass[12pt,a4paper,fleqn]{article}

\paperwidth 597pt
\paperheight 845pt
\voffset -10pt
\hoffset 15pt
\topmargin -3pt
\headheight 0pt
\headsep 0pt
\topskip 0pt
\oddsidemargin -10pt
\evensidemargin 10pt
\textwidth 460pt
\textheight 710pt
\footskip 20pt
\marginparsep 10pt
\marginparwidth 20pt
\marginparpush 5pt
\usepackage[dvips]{graphicx}
\usepackage{amsmath,amssymb}
\usepackage{amsthm}
\usepackage{bm}

% \usepackage{cite}

\allowdisplaybreaks
\begin{document}
\large
\begin{align*}
& x^2+2\sqrt{3}xy-y^2=3 \\
& \Rightarrow (x+\sqrt{3}y)^2-4y^2=3 \\
& {\mathrm{Let}}\; \begin{cases}
	u=x+\sqrt{3}y \\
	v=2y
	\end{cases} \\
& {\mathrm{Then}}\; u^2-v^2=3 \tag{1} \\
& x^2+y^2=(u-\frac{\sqrt{3}}{2}v)^2+\frac{1}{4}v^2=u^2-\sqrt{3}uv+v^2 \tag{2}
\end{align*}

Transform Eq.(1) into parametric equations:
\begin{equation*}
\begin{cases}
	u=\sqrt{3}\,{\mathrm{sec}}\,t \\
	v=\sqrt{3}\,{\mathrm{tan}}\,t
\end{cases}
\end{equation*}

Eq.(2) becomes: \\
\begin{align*}
& \frac{3}{{\mathrm{cos}}^2t}-\frac{3\sqrt{3}\,{\mathrm{sin}}\,t}{{\mathrm{cos}}^2t}+\frac{3\,{\mathrm{sin}}^2t}{{\mathrm{cos}}^2t} \\
& =\frac{3-3\sqrt{3}\,{\mathrm{sin}}\,t+3\,{\mathrm{sin}}^2t}{1-{\mathrm{sin}}\,2t} \tag{3}
\end{align*}

Let $q={\mathrm{sin}}\,t$, Eq.(3)\; becomes:
\begin{align*}
& f(q)=\frac{3-3\sqrt{3}q+3q^2}{1-q^2} \\
& f'(q)=\frac{-3\sqrt{3}q^2+12q-3\sqrt{3}}{(1-q^2)^2}
\end{align*}

For numerator:
\begin{equation*}
\frac{12}{6\sqrt{3}}>1 \\
\end{equation*}

Roots of the numerator are $q_1=\frac{1}{\sqrt{3}}<1$, $q_2=\sqrt{3}>1$

Thus $f(q)$ decreases at $(-1,\frac{1}{\sqrt{3}}]$, increases at $(\frac{1}{\sqrt{3}},1)$

The minimum of $f(q)$, or $x^2+y^2$ is $f(\frac{1}{\sqrt{3}})=\frac{3}{2}$
	
\end{document}